Combine two contexts into one

common.v
@@ -1,13 +1,14 @@
-From WR Require Import syntax.
-From Coq Require Import ssreflect ssrbool List.
-Require Import Psatz.
-From Hammer Require Import Tactics.
+From WR Require Export syntax.
+From Coq Require Export ssreflect ssrbool.
+From mathcomp Require Export zify.
+Export seq.
+From Hammer Require Export Tactics.
 
 Module Type common_sig
   (Import grade : grade_sig)
   (Import syntax : syntax_sig grade).
 
-Notation eith Ξ i := (nth i Ξ el).
+Notation eith Ξ i := (nth el Ξ i).
 
 Definition is_bool_val a :=
   match a with
@@ -16,35 +17,41 @@ Definition is_bool_val a :=
   | _ => false
   end.
 
-Definition context := list tm.
+Definition context := list (grade * tm).
 
 Definition econtext := list grade.
 
-Fixpoint dep_ith Γ i :=
+Definition levels : context -> econtext := seq.unzip1.
+
+Fixpoint dep_ith (Γ : list tm) i :=
   match Γ , i with
   | (A :: Γ), 0 => ren_tm shift A
-  | (A :: Γ), (S i) => ren_tm shift (dep_ith Γ i)
+  | (_ :: Γ), (S i) => ren_tm shift (dep_ith Γ i)
   | _, _ => tFalse
   end.
 
-Notation ith Γ i := (nth i Γ tFalse).
+Notation ith Γ i := (nth tFalse Γ i).
 
-Lemma dep_ith_ren_tm (Γ : context) (A : tm) (x : fin) :
+Lemma dep_ith_ren_tm (Γ : list tm) (A : tm) (x : fin) :
   dep_ith (A :: Γ) (S x) = ren_tm shift (dep_ith Γ x).
 Proof. done. Qed.
 
-Lemma dep_ith_ren_tm0 (Γ : context) (A : tm) :
+Lemma dep_ith_ren_tm0 (Γ : list tm) (A : tm) :
   dep_ith (A :: Γ) 0 = ren_tm shift A.
 Proof. done. Qed.
 
-Definition good_renaming ξ Γ Ξ Δ Ξ' :=
-  forall i, i < length Γ -> ξ i < length Δ /\ dep_ith Δ (ξ i) = ren_tm ξ (dep_ith Γ i) /\ (eith Ξ' (ξ i) <= eith Ξ i)%O.
+Definition good_renaming ξ Γ Δ :=
+  let Γ_ty := seq.unzip2 Γ in
+  let Γ_ℓ := seq.unzip1 Γ in
+  let Δ_ty := seq.unzip2 Δ in
+  let Δ_ℓ := seq.unzip1 Δ in
+  forall i, i < seq.size Γ -> ξ i < seq.size Δ /\ dep_ith Δ_ty (ξ i) = ren_tm ξ (dep_ith Γ_ty i) /\ (eith Δ_ℓ (ξ i) <= eith Γ_ℓ i)%O.
 
 Lemma dep_ith_shift Γ i :
   dep_ith Γ i = ren_tm (Nat.add (S i)) (ith Γ i).
 Proof.
   elim : Γ i.
-  - hauto q:on.
+  - hauto lq:on inv:nat.
   - move => A Γ h.
     case => [|i].
     + done.
@@ -53,31 +60,24 @@ Proof.
       by asimpl.
 Qed.
 
-Lemma list_ith_skipn {A : Type} (a : A)
-  n i (Γ : list A) :
-  nth i (skipn n Γ) a = nth (n + i) Γ a.
-Proof.
-  elim : Γ n i.
-  - hauto lq:on inv:nat.
-  - qauto l:on inv:nat.
-Qed.
+Lemma ith_skipn n i (Γ : list tm) :
+  ith (drop n Γ) i = ith Γ (n + i).
+Proof. by rewrite nth_drop. Qed.
 
-Lemma ith_skipn n i (Γ : context) :
-  ith (skipn n Γ) i = ith Γ (n + i).
-Proof. sfirstorder use:list_ith_skipn.  Qed.
+Lemma eith_skipn n i (Γ : list grade) :
+  eith (drop n Γ) i = eith Γ (n + i).
+Proof. by rewrite nth_drop. Qed.
 
-Lemma eith_skipn n i (Γ : econtext) :
-  eith (skipn n Γ) i = eith Γ (n + i).
-Proof. sfirstorder use:list_ith_skipn. Qed.
-
-Lemma good_renaming_truncate n Γ Ξ :
-  good_renaming (Nat.add n) (skipn n Γ) (skipn n Ξ) Γ Ξ.
+Lemma good_renaming_truncate n Γ :
+  good_renaming (Nat.add n) (drop n Γ) Γ.
 Proof.
   rewrite /good_renaming => i h /=.
   repeat rewrite dep_ith_shift.
+  rewrite /unzip1 /unzip2.
+  repeat rewrite map_drop.
   repeat rewrite ith_skipn eith_skipn.
   split.
-  - rewrite skipn_length in h.
+  - rewrite size_drop in h.
     lia.
   - split.
     + asimpl.
