typing.v
@@ -1,4 +1,4 @@
-From WR Require Import syntax join common.
+From WR Require Export common join.
 
 Module Type typing_sig
   (Import grade : grade_sig)
@@ -6,77 +6,77 @@ Module Type typing_sig
   (Import common : common_sig grade syntax)
   (Import join : join_sig grade syntax common).
 
-Inductive Wt (Γ : context) (Ξ : econtext) : grade -> tm -> tm -> Prop :=
+Inductive Wt (Γ : context) : grade -> tm -> tm -> Prop :=
 | T_Var ℓ i :
-  Wff Γ Ξ ->
-  i < length Γ ->
+  Wff Γ ->
+  i < size Γ ->
+  (eith (unzip1 Γ) i <= ℓ)%O ->
   (* ------ *)
-  Wt Γ Ξ ℓ (var_tm i) (dep_ith Γ i)
+  Wt Γ ℓ (var_tm i) (dep_ith (unzip2 Γ) i)
 
 | T_False ℓ i :
-  Wff Γ Ξ ->
+  Wff Γ ->
   (* -------- *)
-  Wt Γ Ξ ℓ tFalse (tUniv i)
+  Wt Γ ℓ tFalse (tUniv i)
 
 | T_Pi ℓ ℓ0 i A B :
-  Wt Γ Ξ ℓ A (tUniv i) ->
-  Wt (A :: Γ) (ℓ0 :: Ξ) ℓ B (tUniv i) ->
+  Wt Γ ℓ A (tUniv i) ->
+  Wt ((ℓ0, A) :: Γ) ℓ B (tUniv i) ->
   (* --------------------- *)
-  Wt Γ Ξ ℓ (tPi ℓ0 A B) (tUniv i)
+  Wt Γ ℓ (tPi ℓ0 A B) (tUniv i)
 
 | T_Abs ℓ ℓ0 ℓ1 A a B i :
-  Wt Γ Ξ ℓ1 (tPi ℓ0 A B) (tUniv i) ->
-  Wt (A :: Γ) (ℓ0 :: Ξ) ℓ a B ->
+  Wt Γ ℓ1 (tPi ℓ0 A B) (tUniv i) ->
+  Wt ((ℓ0, A) :: Γ) ℓ a B ->
   (* -------------------- *)
-  Wt Γ Ξ ℓ (tAbs ℓ0 A a) (tPi ℓ0 A B)
+  Wt Γ ℓ (tAbs ℓ0 A a) (tPi ℓ0 A B)
 
 | T_App ℓ ℓ0 a A B b :
-  Wt Γ Ξ ℓ a (tPi ℓ0 A B) ->
-  Wt Γ Ξ ℓ0 b A ->
+  Wt Γ ℓ a (tPi ℓ0 A B) ->
+  Wt Γ ℓ0 b A ->
   (* -------------------- *)
-  Wt Γ Ξ ℓ (tApp a ℓ0 b) (subst_tm (b..) B)
+  Wt Γ ℓ (tApp a ℓ0 b) (subst_tm (b..) B)
 
 | T_Conv ℓ ℓ1 a A B i :
-  Wt Γ Ξ ℓ a A ->
-  Wt Γ Ξ ℓ1 B (tUniv i) ->
-  icoherent Ξ A B ->
+  Wt Γ ℓ a A ->
+  Wt Γ ℓ1 B (tUniv i) ->
+  icoherent (unzip1 Γ) A B ->
   (* ----------- *)
-  Wt Γ Ξ ℓ a B
+  Wt Γ ℓ a B
 
 | T_On ℓ :
-  Wff Γ Ξ ->
+  Wff Γ ->
   (* --------- *)
-  Wt Γ Ξ ℓ tOn tSwitch
+  Wt Γ ℓ tOn tSwitch
 
 | T_Off ℓ :
-  Wff Γ Ξ ->
+  Wff Γ ->
   (* --------- *)
-  Wt Γ Ξ ℓ tOff tSwitch
+  Wt Γ ℓ tOff tSwitch
 
 | T_If ℓ a b c A :
-  Wt Γ Ξ ℓ a tSwitch ->
-  Wt Γ Ξ ℓ b A ->
-  Wt Γ Ξ ℓ c A ->
+  Wt Γ ℓ a tSwitch ->
+  Wt Γ ℓ b A ->
+  Wt Γ ℓ c A ->
   (* ------------ *)
-  Wt Γ Ξ ℓ (tIf a b c) A
+  Wt Γ ℓ (tIf a b c) A
 
 | T_Switch ℓ i :
-  Wff Γ Ξ ->
+  Wff Γ ->
   (* ----------- *)
-  Wt Γ Ξ ℓ tSwitch (tUniv i)
+  Wt Γ ℓ tSwitch (tUniv i)
 
 | T_Univ ℓ i j :
-  Wff Γ Ξ ->
+  Wff Γ ->
   i < j ->
   (* ------------ *)
-  Wt Γ Ξ ℓ (tUniv i) (tUniv j)
+  Wt Γ ℓ (tUniv i) (tUniv j)
 
-with Wff (Γ : context) (Ξ : econtext) : Prop :=
+with Wff (Γ : context) : Prop :=
 | Wff_intro F G :
-  length Γ = length Ξ ->
-  (forall i, i < length Γ -> Wt (skipn (S i) Γ) (skipn (S i) Ξ) (G i) (ith Γ i) (tUniv (F i))) ->
+  (forall i, i < length Γ -> Wt (drop (S i) Γ) (G i) (ith (unzip2 Γ) i) (tUniv (F i))) ->
   (* ---------------------------------------------------------------- *)
-  Wff Γ Ξ.
+  Wff Γ.
 
 Scheme wt_ind := Induction for Wt Sort Prop
     with wff_ind := Induction for Wff Sort Prop.
